Fix up [lemma_locations_complete]. See msg.
Previously, we had an assumption in proof of
[lemma_locations_complete] that was unprovable since it was false. By
refining the statement that the lemma proves, we no longer need this
false assumption, and are able to prove things. This does come with
the additional cost of a few "observe" assertions in the
[InstrReordering] proofs, but all is well and good :)

vale/code/lib/transformers/Vale.Transformers.Locations.fsti
@@ -82,15 +82,30 @@ val lemma_locations_truly_disjoint :
     (requires (a <> a_change))
     (ensures (eval_location a s == eval_location a (update_location a_change v s)))
 
+(** Filter out things we don't want to compare on two states *)
+let filter_state (s:machine_state) (flags:flags_t) (ok:bool) (trace:list observation) =
+  { s with
+    ms_flags = FunctionalExtensionality.on_dom flag
+        (fun f ->
+           if f = fCarry then
+             s.ms_flags fCarry
+           else if f = fOverflow then
+             s.ms_flags fOverflow
+           else
+             flags f ) ;
+    ms_ok = ok ;
+    ms_trace = trace }
+
 (** The locations cover everything except some very explicitly mentioned parts of the state. *)
 val lemma_locations_complete :
   s1:machine_state ->
   s2:machine_state ->
+  flags:flags_t ->
   ok:bool ->
   trace:list observation ->
   Lemma
     (requires (
         (forall a. eval_location a s1 == eval_location a s2)))
     (ensures (
-        ({s1 with ms_ok = ok; ms_trace = trace}) ==
-        ({s2 with ms_ok = ok; ms_trace = trace})))
+        filter_state s1 flags ok trace ==
+        filter_state s2 flags ok trace))
